Fixed foldstate

theories/Interp/FoldStateT.v
@@ -40,6 +40,8 @@ Definition refine_state {E C M} S
   (g : bool -> C ~> stateT S M) :
   ctree E C ~> stateT S M := refine g.
 
+Typeclasses Opaque fold_state interp_state refine_state.
+
 Section State.
   Variable (S : Type).
   Variant stateE : Type -> Type :=
@@ -320,406 +322,536 @@ Section State.
 
 End State.
 
+Section FoldBind.
+  Variable (S : Type).
+  Context {E F C D : Type -> Type}
+    `{B1 -< D}.
+
+  Lemma fold_state_bind
+    (h : E ~> stateT S (ctree F D))
+    (g : bool -> C ~> stateT S (ctree F D))
+    {A B}
+    (t : ctree E C A) (k : A -> ctree E C B)
+    (s : S) :
+    fold_state h g (t >>= k) s
+      ≅ fold_state h g t s >>= fun st => fold_state h g (k (snd st)) (fst st).
+  Proof.
+    revert s t.
+    coinduction ? IH; intros.
+    rewrite (ctree_eta t).
+    cbn.
+    rewrite unfold_bind.
+    rewrite unfold_fold_state.
+    destruct (observe t) eqn:Hobs; cbn.
+    - rewrite fold_state_ret. rewrite bind_ret_l. cbn.
+      rewrite unfold_fold_state. reflexivity.
+    - rewrite fold_state_vis.
+      cbn.
+      rewrite bind_bind. cbn.
+      upto_bind_eq.
+      rewrite bind_guard.
+      constructor; intros ?; apply IH.
+    - rewrite unfold_fold_state.
+      cbn.
+
+      rewrite bind_bind.
+      upto_bind_eq.
+      rewrite bind_guard.
+      constructor; intros ?; apply IH.
+  Qed.
+
+  Lemma interp_state_bind `{C -< D}
+    (h : E ~> stateT S (ctree F D))
+    {A B}
+    (t : ctree E C A) (k : A -> ctree E C B)
+    (s : S) :
+    interp_state h (t >>= k) s ≅ interp_state h t s >>= fun xs => interp_state h (k (snd xs)) (fst xs).
+  Proof.
+    eapply fold_state_bind.
+  Qed.
+
+  Lemma refine_state_bind `{E -< F}
+    (g : bool -> C ~> stateT S (ctree F D))
+    {A B}
+    (t : ctree E C A) (k : A -> ctree E C B)
+    (s : S) :
+    refine_state g (t >>= k) s ≅ refine_state g t s >>= fun xs => refine_state g (k (snd xs)) (fst xs).
+  Proof.
+    eapply fold_state_bind.
+  Qed.
+
+End FoldBind.
+
 (* Stateful handlers [E ~> stateT S (itree F)] and morphisms
    [E ~> state S] define stateful itree morphisms
    [itree E ~> stateT S (itree F)]. *)
-(* Section State. *)
+From CTree Require Import FoldCTree.
 
-(*   Variable (S : Type). *)
-(*   Context {E F C D : Type -> Type} *)
-(*           `{B1 -< D} *)
-(*           {R : Type} *)
-(*           (h : E ~> stateT S (ctree F D)) *)
-(*           (h' : bool -> C ~> stateT S (ctree F D)). *)
-
-(*   Lemma fold_state_bind {A B} *)
-(*         (t : ctree E C A) (k : A -> ctree E C B) *)
-(*         (s : S) : *)
-(*     (fold_state h h' (t >>= k) s) *)
-(*       ≅ *)
-(*       (fold_state h h' t s >>= fun st => fold_state h h' (k (snd st)) (fst st)). *)
-(*   Proof. *)
-(*     revert s t. *)
-(*     coinduction ? IH; intros. *)
-(*     rewrite (ctree_eta t). *)
-(*     cbn. *)
-(*     rewrite unfold_bind. *)
-(*     rewrite unfold_fold_state. *)
-(*     destruct (observe t) eqn:Hobs; cbn. *)
-(*     - rewrite fold_state_ret. rewrite bind_ret_l. cbn. *)
-(*       rewrite unfold_fold_state. reflexivity. *)
-(*     - rewrite fold_state_vis. *)
-(*       cbn. *)
-(*       rewrite bind_bind. cbn. *)
-(*       upto_bind_eq. *)
-(*       rewrite bind_guard. *)
-(*       constructor; intros ?; apply IH. *)
-(*     - rewrite unfold_fold_state. *)
-(*       cbn. *)
-
-(*       rewrite bind_bind. *)
-(*       upto_bind_eq. *)
-(*       rewrite bind_guard. *)
-(*       constructor; intros ?; apply IH. *)
-(*   Qed. *)
-
-  (** LEF: This looks like it depends on [SBisimInterp.v]? Move there? *)
-  (*
-Lemma trans0_fold_state : forall {E F X} (h : E ~> stateT S (ctree F)) (t t' : ctree E X) s,
-  trans0 t t' -> trans0 (fold_state h t s) (fold_state h t' s).
+(* TODO MOVE *)
+Lemma bind_branch : forall {E C X Y} (c : C Y) (b : bool) (k : Y -> ctree E C X),
+    CTree.branch b c >>= k ≅ Br b c k.
 Proof.
-  intros. red in H. setoid_rewrite (ctree_eta t). setoid_rewrite (ctree_eta t').
-  genobs t ot. genobs t' ot'. clear t Heqot t' Heqot'.
-  induction H.
-  - constructor. rewrite H. reflexivity.
-  - rewrite unfold_fold_state. cbn.
-    apply T0Br with (x := x).
-    apply T0Br with (x := Fin.F1). apply IHtrans0_.
+  intros; cbn; unfold CTree.branch; rewrite bind_br; step; constructor; intros ?; now rewrite bind_ret_l.
 Qed.
 
-(* transi *)
-
-Inductive transi_state {E F X} (h : E ~> stateT S (ctree F)) : @label F -> S -> S -> ctree E X -> ctree E X -> Prop :=
-| transis_val : forall (x : X) t t' s,
-    trans (val x) t t' ->
-    transi_state h (val (s, x)) s s t t'
-| transis_tau : forall t t' s,
-    trans tau t t' ->
-    transi_state h tau s s t t'
-| transis_obs : forall Y (e : E Y) x l t t' t'' s s',
-    trans (obs e x) t t' ->
-    t0_det t'' (Ret (s', x)) ->
-    trans l (h _ e s) t'' ->
-    transi_state h l s s' t t'
-| transis_obs0 : forall Y (e : E Y) l x t t' t'' s s' s'',
-    trans (obs e x) t t' ->
-    transi_state h l s' s'' t' t'' ->
-    trans (val (s', x)) (h _ e s) CTree.stuckD ->
-    transi_state h l s s'' t t''
-.
-
-#[global] Instance transis_equ :
-  forall {E F X} (h : E ~> stateT S (ctree F)) l s s',
-  Proper (equ eq ==> equ eq ==> flip impl) (@transi_state E F X h l s s').
-Proof.
-  cbn. intros.
-  revert x x0 H H0. induction H1; intros.
-  - apply transis_val. rewrite H0, H1. apply H.
-  - apply transis_tau. rewrite H0, H1. apply H.
-  - rewrite <- H2, <- H3 in *. eapply transis_obs; eauto.
-  - rewrite <- H2 in *. eapply transis_obs0; eauto.
-Qed.
-
-#[global] Instance transis_equ' :
-  forall {E F X} (h : E ~> stateT S (ctree F)) l s s',
-  Proper (equ eq ==> equ eq ==> impl) (@transi_state E F X h l s s').
-Proof.
-  cbn. intros. rewrite <- H, <- H0. apply H1.
-Qed.
-
-Lemma transis_brD {E F X} (h : E ~> stateT S (ctree F)) : forall l s s' (t' : ctree E X) n k x,
-  transi_state h l s s' (k x) t' ->
-  transi_state h l s s' (BrD n k) t'.
-Proof.
-  intros. inv H.
-  - apply transis_val. etrans.
-  - apply transis_tau. etrans.
-  - eapply transis_obs; etrans.
-  - eapply transis_obs0; etrans.
-Qed.
-
-Lemma trans0_transi {E F X} (h : E ~> stateT S (ctree F)) :
-  forall l s s' (t t' t'' : ctree E X), trans0 t t' -> transi_state h l s s' t' t'' -> transi_state h l s s' t t''.
+Lemma trans_branch :
+  forall {E B : Type -> Type} {X : Type} {H : B0 -< B} {Y : Type}
+    [l : label] [t t' : ctree E B X] (c : B Y) (k : Y -> ctree E B X) (x : Y),
+    trans l t t' -> k x ≅ t -> trans l (CTree.branch false c >>= k) t'.
 Proof.
   intros.
-  red in H. rewrite (ctree_eta t). rewrite (ctree_eta t') in H0.
-  genobs t ot. genobs t' ot'. clear t Heqot. clear t' Heqot'.
-  revert l t'' H0. induction H; intros.
-  - rewrite H. apply H0.
-  - eapply transis_brD. setoid_rewrite <- ctree_eta in IHtrans0_. apply IHtrans0_. apply H0.
+  rewrite bind_branch.
+  eapply trans_brD; eauto.
 Qed.
 
-Lemma transis_sbisim {E F X} (h : E ~> stateT S (ctree F)) :
-  forall l s s' (t t' u : ctree E X), transi_state h l s s' t t' ->
-  t ~ u ->
-  exists u', transi_state h l s s' u u' /\ t' ~ u'.
-Proof.
-  intros. revert u H0.
-  induction H; intros.
-  - step in H0. destruct H0 as [? _]. apply H0 in H. destruct H.
-    exists x0. split. now apply transis_val. apply H1.
-  - step in H0. destruct H0 as [? _]. apply H0 in H. destruct H.
-    exists x. split. now apply transis_tau. apply H1.
-  - step in H2. destruct H2 as [? _]. apply H2 in H. destruct H.
-    exists x0. split. eapply transis_obs; eauto. apply H3.
-  - step in H2. destruct H2 as [? _]. apply H2 in H. destruct H.
-    apply IHtransi_state in H3 as (? & ? & ?). exists x1.
-    split. eapply transis_obs0; eauto. apply H4.
-Qed.
+Section transi_state.
 
-Lemma transis_trans {E F X} (h : E ~> stateT S (ctree F)) (Hh : forall X e s, vsimple (h X e s)) :
-  forall l s s' (t t' : ctree E X),
-  transi_state h l s s' t t' -> exists t0, trans l (fold_state h t s) t0 /\ t0_det t0 (fold_state h t' s').
-Proof.
-  intros. induction H.
-  - exists CTree.stuckD. apply trans_val_inv in H as ?.
-    apply trans_val_trans0 in H as [].
-    eapply trans0_fold_state in H. rewrite fold_state_ret in H. setoid_rewrite H0.
-    setoid_rewrite fold_state_br. setoid_rewrite br0_always_stuck.
-    eapply trans0_trans in H; etrans. split; etrans. now left.
-  - exists (Guard (fold_state h t' s)). split; [| eright; eauto; now left ].
-    apply trans_tau_trans0 in H as (? & ? & ? & ? & ?).
-    eapply trans0_fold_state in H. setoid_rewrite H0. eapply trans0_trans; etrans.
-    setoid_rewrite fold_state_br.
-    econstructor. reflexivity.
-  - exists (x <- t'';; Guard (fold_state h t' s')).
-    split. 2: { eapply t0_det_bind_ret_l; eauto. eright; eauto. now left. }
-    apply trans_obs_trans0 in H as (? & ? & ?).
-    eapply trans0_fold_state in H. setoid_rewrite H2. eapply trans0_trans; etrans.
-    setoid_rewrite fold_state_vis.
-    eapply trans_bind_l with (k := fun sx => Guard (fold_state h (x0 (snd sx)) (fst sx))) in H1.
-    setoid_rewrite t0_det_bind_ret_l_equ in H1 at 2; eauto. cbn in *. eapply H1.
-    { intro. inv H3. apply trans_val_inv in H1. rewrite H1 in H0. inv H0. step in H3. inv H3. step in H4. inv H4. }
-  - destruct IHtransi_state as (? & ? & ?).
-    destruct (Hh Y e s). 2: { destruct H4. rewrite H4 in H1. apply trans_vis_inv in H1 as (? & ? & ?). step in H1. inv H1. }
-    destruct H4. rewrite H4 in H1. inv_trans. subst.
-    exists x0. split. 2: auto.
-    apply trans_obs_trans0 in H as (? & ? & ?). eapply trans0_fold_state in H.
-    setoid_rewrite fold_state_vis in H. setoid_rewrite H4 in H. setoid_rewrite bind_ret_l in H.
-    eapply trans0_trans; etrans. setoid_rewrite <- H1. etrans.
-Qed.
+  Variable S : Type.
+  Context {E F C D : Type -> Type}
+    `{CST1 : B0 -< C} {CST2 : C -< D} `{CST3 : B1 -< D} `{CST4 : E -< F}.
+  Context {X : Type}.
+  Variable (h : E ~> stateT S (ctree F D)).
 
-(** Various lemmas for the proof that fold_state preserves sbisim in some cases. *)
+  Lemma trans0_interp_state : forall (t t' : ctree E C X) s,
+      trans0 t t' ->
+      trans0 (interp_state h t s) (interp_state h t' s).
+  Proof.
+    intros; red in H.
+    rewrite (ctree_eta t), (ctree_eta t').
+    genobs t ot. genobs t' ot'. clear t Heqot t' Heqot'.
+    induction H.
+    - constructor. rewrite H. reflexivity.
+    - rewrite unfold_interp_state. cbn.
+      rewrite bind_bind.
+      unfold mbr, MonadBr_ctree, CTree.branch.
+      rewrite bind_br.
+      eapply T0Br with (x := x).
+      rewrite !bind_ret_l.
+      cbn.
+      eapply T0Br with (x := tt).
+      apply IHtrans0_.
+  Qed.
 
-Lemma fold_state_ret_inv {E F X} (h : E ~> stateT S (ctree F)) : forall s (t : ctree E X) r,
-  fold_state h t s ≅ Ret r -> t ≅ Ret (snd r) /\ s = fst r.
-Proof.
-  intros. setoid_rewrite (ctree_eta t) in H. setoid_rewrite (ctree_eta t).
-  destruct (observe t) eqn:?.
-  - rewrite fold_state_ret in H. step in H. inv H. split; reflexivity.
-  - rewrite fold_state_vis in H. apply ret_equ_bind in H as (? & ? & ?). step in H0. inv H0.
-  - rewrite fold_state_br in H. step in H. inv H.
-Qed.
+  (* transi *)
 
-Lemma trans_fold_state_inv_gen {E F X Y} (h : E ~> stateT S (ctree F)) (Hh : forall X e s, vsimple (h X e s)) :
-  forall l s (k : Y -> ctree E X) t' (pre : ctree F Y),
-  is_simple pre ->
-  trans l (x <- pre;; fold_state h (k x) s) t' ->
-  exists t0 s', t0_det t' (fold_state h t0 s') /\
-  ((exists l t1 x, trans l pre t1 /\ t0_det t1 (Ret x : ctree F Y) /\ t0 ≅ k x) \/
-    exists (x : Y), trans (val x) pre CTree.stuckD /\ trans l (fold_state h (k x) s) t' /\ transi_state h l s s' (k x) t0).
-Proof.
-  intros * Hpre H.
-  do 3 red in H. remember (observe (x <- pre;; fold_state h (k x) s)) as oi.
-  setoid_rewrite (ctree_eta t') at 1.
-  setoid_rewrite (ctree_eta t') at 2.
-  genobs t' ot'. clear t' Heqot'.
-  assert (go oi ≅ x <- pre;; fold_state h (k x) s).
-  { rewrite Heqoi, <- ctree_eta. reflexivity. } clear Heqoi.
-  revert Y s k pre Hpre H0. induction H; intros.
-  - destruct n. now apply Fin.case0.
-    symmetry in H0. apply br_equ_bind in H0 as ?.
-    destruct H1 as [[] | (? & ? & ?)].
-    + rewrite H1 in H0. setoid_rewrite bind_ret_l in H0. setoid_rewrite H1. clear pre Hpre H1.
-      rewrite (ctree_eta (k0 x0)) in H0. destruct (observe (k0 x0)) eqn:?.
-      * rewrite fold_state_ret in H0. step in H0. inv H0.
-      * rewrite fold_state_vis in H0. apply br_equ_bind in H0 as ?. destruct H1 as [[] | (? & ? & ?)].
-        --setoid_rewrite H1 in H0. setoid_rewrite bind_ret_l in H0.
-          apply equ_br_invT in H0 as ?. destruct H2 as [? _]. apply eq_add_S in H2 as <-.
-          simple apply equ_br_invE with (x := x) in H0.
-          rewrite <- H0 in H.
-          specialize (IHtrans_ _ (fst x1) (fun (_ : unit) => k1 (snd x1)) (Ret tt)).
-          edestruct IHtrans_ as (? & ? & ?).
-          { apply is_simple_ret. }
-          { rewrite <- ctree_eta. setoid_rewrite bind_ret_l. setoid_rewrite H0. reflexivity. }
-          destruct H2. exists x2, x3. split; auto. right. destruct H3.
-          { destruct H3 as (? & ? & ? & ? & ? & ?). inv_trans. subst.
-            inv H4. step in H3. inv H3. step in H6. inv H6. }
-          destruct H3 as (_ & _ & ? & ?). exists x0. split. etrans. split.
-          ++setoid_rewrite (ctree_eta (k0 x0)). rewrite Heqc.
-            setoid_rewrite fold_state_vis. setoid_rewrite H1. setoid_rewrite bind_ret_l. apply trans_guard. apply H3.
-          ++setoid_rewrite (ctree_eta (k0 x0)). rewrite Heqc. destruct x1.
-             eapply transis_obs0. etrans. 2: { rewrite H1. etrans. } cbn in H4. cbn in *. etrans.
-        --destruct (Hh X0 e s).
-          destruct H3. rewrite H3 in H1. step in H1. inv H1.
-          destruct H3. rewrite H3 in H1. step in H1. inv H1.
-      * rewrite fold_state_br in H0.
-        apply equ_br_invT in H0 as ?. destruct H1 as [-> ->].
-        simple apply equ_br_invE with (x := x) in H0 as ?.
-        specialize (IHtrans_ _ s (fun _ : unit => k1 x) (Guard (Ret tt))).
+  Instance foo : B0 -< D.
+  intros ? ?; now apply CST2, CST1.
+  Defined.
+
+  Inductive transi_state : @label F -> S -> S -> ctree E C X -> ctree E C X -> Prop :=
+  | transis_val : forall (x : X) t t' s,
+      trans (val x) t t' ->
+      transi_state (val (s, x)) s s t t'
+  | transis_tau : forall t t' s,
+      trans tau t t' ->
+      transi_state tau s s t t'
+  | transis_obs : forall Y (e : E Y) x l t t' t'' s s',
+      trans (obs e x) t t' ->
+      t0_det t'' (Ret (s', x)) ->
+      trans l (h e s) t'' ->
+      transi_state l s s' t t'
+  | transis_obs0 : forall Y (e : E Y) l x t t' t'' s s' s'',
+      trans (obs e x) t t' ->
+      transi_state l s' s'' t' t'' ->
+      trans (val (s', x)) (h e s) stuckD ->
+      transi_state l s s'' t t''
+  .
+
+  #[global] Instance transis_equ :
+    forall l s s',
+      Proper (equ eq ==> equ eq ==> flip impl) (@transi_state l s s').
+  Proof.
+    cbn. intros.
+    revert x x0 H H0. induction H1; intros.
+    - apply transis_val. rewrite H0, H1. apply H.
+    - apply transis_tau. rewrite H0, H1. apply H.
+    - rewrite <- H2, <- H3 in *. eapply transis_obs; eauto.
+    - rewrite <- H2 in *. eapply transis_obs0; eauto.
+  Qed.
+
+  #[global] Instance transis_equ' :
+    forall l s s',
+      Proper (equ eq ==> equ eq ==> impl) (@transi_state l s s').
+  Proof.
+    cbn. intros. rewrite <- H, <- H0. apply H1.
+  Qed.
+
+  Lemma transis_brD : forall Y l s s' (t' : ctree E C X) (c : C Y) k x,
+      transi_state l s s' (k x) t' ->
+      transi_state l s s' (BrD c k) t'.
+  Proof.
+    intros. inv H.
+    - apply transis_val. etrans.
+    - apply transis_tau. etrans.
+    - eapply transis_obs; etrans.
+    - eapply transis_obs0; etrans.
+  Qed.
+
+  Lemma trans0_transi :
+    forall l s s' (t t' t'' : ctree E C X),
+      trans0 t t' ->
+      transi_state l s s' t' t'' ->
+      transi_state l s s' t t''.
+  Proof.
+    intros.
+    red in H. rewrite (ctree_eta t). rewrite (ctree_eta t') in H0.
+    genobs t ot. genobs t' ot'. clear t Heqot. clear t' Heqot'.
+    revert l t'' H0. induction H; intros.
+    - rewrite H. apply H0.
+    - eapply transis_brD. setoid_rewrite <- ctree_eta in IHtrans0_. apply IHtrans0_. apply H0.
+  Qed.
+
+  Lemma transis_sbisim :
+    forall l s s' (t t' u : ctree E C X),
+      transi_state l s s' t t' ->
+      t ~ u ->
+      exists u', transi_state l s s' u u' /\ t' ~ u'.
+  Proof.
+    intros. revert u H0.
+    induction H; intros.
+    - step in H0. destruct H0 as [? _]. apply H0 in H.
+      destruct H as (? & ? & ? & ? & ?); subst.
+      eexists. split. eapply transis_val; eauto. apply H1.
+    - step in H0. destruct H0 as [? _]. apply H0 in H.
+      destruct H as (? & ? & ? & ? & ?); subst.
+      eexists. split. eapply transis_tau; eauto. apply H1.
+    - step in H2. destruct H2 as [? _]. apply H2 in H.
+      destruct H as (? & ? & ? & ? & ?); subst.
+      eexists. split. eapply transis_obs; eauto. apply H3.
+    - step in H2. destruct H2 as [? _]. apply H2 in H.
+      destruct H as (? & ? & ? & ? & ?); subst.
+      apply IHtransi_state in H3 as (? & ? & ?).
+      eexists; split. eapply transis_obs0; eauto. apply H4.
+  Qed.
+
+  Lemma transis_trans (Hh : forall X (e : _ X) s, vsimple (h e s)) :
+    forall l s s' (t t' : ctree E C X),
+      transi_state l s s' t t' ->
+      exists t0, trans l (interp_state h t s) t0 /\ t0_det t0 (interp_state h t' s').
+  Proof.
+    intros. induction H.
+    - exists stuckD. apply trans_val_inv in H as ?.
+      apply trans_val_trans0 in H as [].
+      eapply trans0_interp_state in H. rewrite interp_state_ret in H. setoid_rewrite H0.
+      setoid_rewrite interp_state_br.
+      split.
+      eapply trans0_trans in H; etrans.
+      left.
+      rewrite bind_branch.
+      step.
+      constructor; intros [].
+
+    - exists (Guard (interp_state h t' s)). split; [| eright; eauto; now left ].
+      apply trans_tau_trans0 in H as (? & ? & ? & ? & ? & ?).
+      eapply trans0_interp_state in H. setoid_rewrite H0. eapply trans0_trans; etrans.
+      rewrite interp_state_br, bind_branch.
+      econstructor. reflexivity.
+    - exists (x <- t'';; Guard (interp_state h t' s')).
+      split.
+      2: { eapply t0_det_bind_ret_l; eauto. eright; eauto. now left. }
+      apply trans_obs_trans0 in H as (? & ? & ?).
+      eapply trans0_interp_state in H. setoid_rewrite H2. eapply trans0_trans; etrans.
+      setoid_rewrite interp_state_vis.
+      eapply trans_bind_l with (k := fun sx => Guard (interp_state h (x0 (snd sx)) (fst sx))) in H1.
+      setoid_rewrite t0_det_bind_ret_l_equ in H1 at 2; eauto. cbn in *. eapply H1.
+      { intro. inv H3. apply trans_val_inv in H1. rewrite H1 in H0. inv H0. step in H3. inv H3. step in H4. inv H4. auto using void_unit_elim. }
+    - destruct IHtransi_state as (? & ? & ?).
+      destruct (Hh Y e s).
+      2: { destruct H4. rewrite H4 in H1. apply trans_vis_inv in H1 as (? & ? & ?). step in H1. inv H1. }
+      destruct H4. rewrite H4 in H1. inv_trans. subst.
+      exists x0. split. 2: auto.
+      apply trans_obs_trans0 in H as (? & ? & ?). eapply trans0_interp_state in H.
+      setoid_rewrite interp_state_vis in H. setoid_rewrite H4 in H. setoid_rewrite bind_ret_l in H.
+      eapply trans0_trans; etrans. setoid_rewrite <- H1. etrans.
+  Qed.
+
+  Lemma interp_state_ret_inv :
+    forall s (t : ctree E C X) r,
+      interp_state h t s ≅ Ret r -> t ≅ Ret (snd r) /\ s = fst r.
+  Proof.
+    intros. setoid_rewrite (ctree_eta t) in H. setoid_rewrite (ctree_eta t).
+    destruct (observe t) eqn:?.
+    - rewrite interp_state_ret in H. step in H. inv H. split; reflexivity.
+    - rewrite interp_state_vis in H. apply ret_equ_bind in H as (? & ? & ?). step in H0. inv H0.
+    - rewrite interp_state_br in H. step in H. inv H.
+  Qed.
+
+  Lemma trans_interp_state_inv_gen (Hh : forall X (e : _ X) s, vsimple (h e s)) :
+    forall Y l s (k : Y -> ctree E C X) t' (pre : ctree F D Y),
+      is_simple pre ->
+      trans l (x <- pre;; interp_state h (k x) s) t' ->
+      exists t0 s', t0_det t' (interp_state h t0 s') /\
+                 ((exists l t1 x, trans l pre t1 /\ t0_det t1 (Ret x : ctree F D Y) /\ t0 ≅ k x) \/
+                    exists (x : Y), trans (val x) pre stuckD /\ trans l (interp_state h (k x) s) t' /\ transi_state l s s' (k x) t0).
+  Proof.
+    intros * Hpre H.
+    do 3 red in H. remember (observe (x <- pre;; interp_state h (k x) s)) as oi.
+    setoid_rewrite (ctree_eta t') at 1.
+    setoid_rewrite (ctree_eta t') at 2.
+    genobs t' ot'. clear t' Heqot'.
+    assert (go oi ≅ x <- pre;; interp_state h (k x) s).
+    { rewrite Heqoi, <- ctree_eta. reflexivity. } clear Heqoi.
+    revert Y s k pre Hpre H0. induction H; intros.
+    - symmetry in H0. apply br_equ_bind in H0 as ?.
+      destruct H1 as [[] | (? & ? & ?)].
+      + rewrite H1 in H0. setoid_rewrite bind_ret_l in H0. setoid_rewrite H1. clear pre Hpre H1.
+        rewrite (ctree_eta (k0 x0)) in H0. destruct (observe (k0 x0)) eqn:?.
+        * rewrite interp_state_ret in H0. step in H0. inv H0.
+        * rewrite interp_state_vis in H0. apply br_equ_bind in H0 as ?. destruct H1 as [[] | (? & ? & ?)].
+          --setoid_rewrite H1 in H0. setoid_rewrite bind_ret_l in H0.
+            apply equ_br_invT in H0 as ?. destruct H2 as [? _]. subst.
+            apply equ_br_invE in H0 as [<- ?].
+            rewrite <- H0 in H.
+            specialize (IHtrans_ _ (fst x1) (fun (_ : unit) => k1 (snd x1)) (Ret tt)).
+            edestruct IHtrans_ as (? & ? & ?).
+            { apply is_simple_ret. }
+            { rewrite <- ctree_eta. setoid_rewrite bind_ret_l. setoid_rewrite H0. reflexivity. }
+            destruct H2. exists x2, x3. split; auto. right. destruct H3.
+            { destruct H3 as (? & ? & ? & ? & ? & ?). inv_trans. subst.
+              inv H4. step in H3. inv H3. step in H6. inv H6.
+              exfalso; now apply void_unit_elim.
+            }
+            destruct H3 as (_ & _ & ? & ?). exists x0. split. etrans. split.
+            ++setoid_rewrite (ctree_eta (k0 x0)). rewrite Heqc0.
+              setoid_rewrite interp_state_vis. setoid_rewrite H1. setoid_rewrite bind_ret_l. apply trans_guard. apply H3.
+            ++setoid_rewrite (ctree_eta (k0 x0)). rewrite Heqc0. destruct x1.
+              eapply transis_obs0. etrans. 2: { rewrite H1. etrans. } cbn in H4. cbn in *. etrans.
+          -- destruct (Hh _ e s).
+             destruct H3. rewrite H3 in H1. step in H1. inv H1.
+             destruct H3. rewrite H3 in H1. step in H1. inv H1.
+        * rewrite interp_state_br in H0.
+          rewrite bind_branch in H0.
+          apply equ_br_invT in H0 as ?. destruct H1 as [-> ->].
+          apply equ_br_invE in H0 as [<- ?].
+          specialize (IHtrans_ _ s (fun _ : unit => k1 x) (Guard (Ret tt))).
+          edestruct IHtrans_ as (? & ? & ? & ?).
+          { apply is_simple_guard_ret. }
+          { rewrite <- ctree_eta. setoid_rewrite bind_br. setoid_rewrite bind_ret_l. now rewrite <- H0. }
+          destruct H2.
+          { destruct H2 as (? & ? & ? & ? & ? & ?). inv_trans. subst.
+            inv H3. step in H2. inv H2. step in H4. inv H4.
+            exfalso; now apply void_unit_elim.
+          }
+          destruct H2 as (? & ? & ? & ?).
+          exists x1, x2. split; auto. right. exists x0. split; etrans. split.
+          rewrite (ctree_eta (k0 x0)), Heqc0, interp_state_br.
+          eapply trans_branch.
+          2: reflexivity. apply trans_guard. apply H3.
+          rewrite (ctree_eta (k0 x0)), Heqc0. eapply transis_brD; etrans.
+      + specialize (IHtrans_ _ s k0 (x0 x)).
         edestruct IHtrans_ as (? & ? & ? & ?).
-        { apply is_simple_guard_ret. }
-        { rewrite <- ctree_eta. setoid_rewrite bind_br. setoid_rewrite bind_ret_l. now rewrite H1. }
-        destruct H3.
-        { destruct H3 as (? & ? & ? & ? & ? & ?). inv_trans. subst.
-          inv H4. step in H3. inv H3. step in H5. inv H5. }
-        destruct H3 as (? & ? & ? & ?).
-        exists x1, x2. split; auto. right. exists x0. split; etrans. split.
-        rewrite (ctree_eta (k0 x0)), Heqc, fold_state_br.
-        eapply trans_brD. 2: reflexivity. apply trans_guard. apply H4.
-        rewrite (ctree_eta (k0 x0)), Heqc. eapply transis_brD; etrans.
-    + specialize (IHtrans_ _ s k0 (x0 x)).
-      edestruct IHtrans_ as (? & ? & ? & ?).
-      { apply is_simple_brD. red. setoid_rewrite <- H1. apply Hpre. }
-      rewrite <- ctree_eta. apply H2. destruct H4 as [(? & ? & ? & ? & ? & ?) | (? & ? & ? & ?)].
+        { eapply is_simple_brD. red. setoid_rewrite <- H1. apply Hpre. }
+        rewrite <- ctree_eta. apply H2. destruct H4 as [(? & ? & ? & ? & ? & ?) | (? & ? & ? & ?)].
         exists (k0 x5), x2. split. { now rewrite H6 in H3. }
         left. eapply trans_brD in H4. 2: reflexivity. rewrite <- H1 in H4. eauto 6.
-      * exists x1, x2. split; auto. right. exists x3. rewrite H1. etrans.
-  - destruct n. now apply Fin.case0.
-    symmetry in H0. apply br_equ_bind in H0 as ?. destruct H1 as [[] | (? & ? & ?)].
-    + rewrite H1 in H0. setoid_rewrite bind_ret_l in H0.
-      rewrite (ctree_eta (k0 x0)) in H0. destruct (observe (k0 x0)) eqn:?.
-      * rewrite fold_state_ret in H0. step in H0. inv H0.
-      * rewrite fold_state_vis in H0. apply br_equ_bind in H0 as ?.
-        destruct H2 as [[] | (? & ? & ?)].
-        { rewrite H2 in H0. setoid_rewrite bind_ret_l in H0. step in H0. inv H0. }
-        pose proof (trans_brS x1 x). rewrite <- H2 in H4.
-        edestruct Hh. { destruct H5. rewrite H5 in H4. inv_trans. }
-        destruct H5. rewrite H5 in H4. apply trans_vis_inv in H4 as (? & ? & ?). discriminate.
-      * rewrite fold_state_br in H0.
-        apply equ_br_invT in H0 as ?. destruct H2 as [-> ->].
-        simple eapply equ_br_invE in H0 as ?. rewrite H in H2.
-        exists (k1 x), s. symmetry in H2. split.
-        { rewrite <- ctree_eta. rewrite H2. eapply t0_det_tau; auto. apply t0_det_id; auto. }
-        right. exists x0. rewrite H1. split; etrans.
-        split; setoid_rewrite (ctree_eta (k0 x0)); setoid_rewrite Heqc.
-        { setoid_rewrite fold_state_br. rewrite H2.
-          econstructor. now rewrite <- ctree_eta. }
-        econstructor; etrans.
-    + pose proof (trans_brS x0 x).
-      rewrite <- H1 in H3. edestruct Hpre.
-      { apply H4 in H3. inv H3. }
-      apply H4 in H3 as [].
-      specialize (H2 x).
-      exists (k0 x1), s. rewrite H in H2. split.
-      { rewrite <- ctree_eta, H2. eapply t0_det_bind_ret_l; eauto. now left. }
-      left. exists tau, (x0 x), x1. split; auto. rewrite H1. etrans.
-  - symmetry in H0. apply vis_equ_bind in H0 as ?. destruct H1 as [[] | (? & ? & ?)].
-    + rewrite H1 in H0. setoid_rewrite bind_ret_l in H0.
-     rewrite (ctree_eta (k0 x0)) in H0. destruct (observe (k0 x0)) eqn:?.
-      * rewrite fold_state_ret in H0. step in H0. inv H0.
-      * rewrite fold_state_vis in H0. apply vis_equ_bind in H0 as ?.
-        destruct H2 as [[] | (? & ? & ?)].
-        { rewrite H2 in H0. setoid_rewrite bind_ret_l in H0. step in H0. inv H0. }
-        pose proof (trans_vis e x x1). rewrite <- H2 in H4.
-        edestruct Hh. { destruct H5. rewrite H5 in H4. inv H4. }
-        destruct H5. rewrite H5 in H4.
-        specialize (H3 x). rewrite H5 in H2.
-        apply equ_vis_invT in H2 as ?. subst.
-        apply equ_vis_invE in H2 as ?. destruct H6 as [-> ?].
-        rewrite <- H6 in *. rewrite bind_ret_l in H3.
-        exists (k1 (snd x)), (fst x).
-        rewrite H in H3. split. { rewrite <- ctree_eta, H3. eright; eauto. eleft; auto. }
-        right.
-        exists x0. rewrite H1. split; etrans.
-        split; setoid_rewrite (ctree_eta (k0 x0)); setoid_rewrite Heqc.
-        { setoid_rewrite fold_state_vis. rewrite H5. setoid_rewrite bind_vis.
-          econstructor. rewrite bind_ret_l. rewrite <- H3, <- ctree_eta. reflexivity. }
-        eapply transis_obs; etrans. 2: { rewrite H5. etrans. } destruct x. now left.
-      * rewrite fold_state_br in H0. step in H0. inv H0.
-    + pose proof (trans_vis e x x0).
-      rewrite <- H1 in H3. edestruct Hpre.
-      { apply H4 in H3. inv H3. }
-      apply H4 in H3 as [].
-      specialize (H2 x).
-      exists (k0 x1), s. rewrite H in H2. split.
-      { rewrite <- ctree_eta, H2. eapply t0_det_bind_ret_l; eauto. now left. }
-      left. exists (obs e x), (x0 x), x1. split; auto. rewrite H1. etrans.
-     - exists (CTree.stuckD), (fst r). split.
-       + left. unfold CTree.stuckD. rewrite fold_state_br.
-         rewrite !br0_always_stuck. reflexivity.
-       + right. symmetry in H0. apply ret_equ_bind in H0 as (? & ? & ?).
-         exists x. rewrite H. split; etrans. split.
-         rewrite H0. rewrite br0_always_stuck. etrans.
-         apply fold_state_ret_inv in H0 as []. subst. rewrite H0. destruct r. cbn. apply transis_val. econstructor; etrans.
-Qed.
+        * exists x1, x2. split; auto. right. exists x3. rewrite H1. etrans.
+    - symmetry in H0. apply br_equ_bind in H0 as ?. destruct H1 as [[] | (? & ? & ?)].
+      + rewrite H1 in H0. setoid_rewrite bind_ret_l in H0.
+        rewrite (ctree_eta (k0 x0)) in H0. destruct (observe (k0 x0)) eqn:?.
+        * rewrite interp_state_ret in H0. step in H0. inv H0.
+        * rewrite interp_state_vis in H0. apply br_equ_bind in H0 as ?.
+          destruct H2 as [[] | (? & ? & ?)].
+          { rewrite H2 in H0. setoid_rewrite bind_ret_l in H0. step in H0. inv H0. }
+          pose proof (trans_brS c x1 x). rewrite <- H2 in H4.
+          edestruct Hh. { destruct H5. rewrite H5 in H4. inv_trans. }
+          destruct H5. rewrite H5 in H4. apply trans_vis_inv in H4 as (? & ? & ?). discriminate.
+        * rewrite interp_state_br in H0.
+          rewrite bind_branch in H0.
+          apply equ_br_invT in H0 as ?. destruct H2 as [-> ->].
+          simple eapply equ_br_invE in H0 as ?. destruct H2 as [<- ?].
+          specialize (H2 x). rewrite H in H2.
+          exists (k1 x), s. symmetry in H2. split.
+          { rewrite <- ctree_eta. rewrite H2. eapply t0_det_tau; auto. apply t0_det_id; auto. }
+          right. exists x0. rewrite H1. split; etrans.
+          split; setoid_rewrite (ctree_eta (k0 x0)); setoid_rewrite Heqc0.
+          { setoid_rewrite interp_state_br. rewrite H2.
+            rewrite bind_branch.
+            econstructor. now rewrite <- ctree_eta. }
+          econstructor; etrans.
+      + pose proof (trans_brS c x0 x).
+        rewrite <- H1 in H3. edestruct Hpre.
+        { apply H4 in H3. inv H3. }
+        apply H4 in H3 as [].
+        specialize (H2 x).
+        exists (k0 x1), s. rewrite H in H2. split.
+        { rewrite <- ctree_eta, H2. eapply t0_det_bind_ret_l; eauto. now left. }
+        left. exists tau, (x0 x), x1. split; auto. rewrite H1. etrans.
+    - symmetry in H0. apply vis_equ_bind in H0 as ?. destruct H1 as [[] | (? & ? & ?)].
+      + rewrite H1 in H0. setoid_rewrite bind_ret_l in H0.
+        rewrite (ctree_eta (k0 x0)) in H0. destruct (observe (k0 x0)) eqn:?.
+        * rewrite interp_state_ret in H0. step in H0. inv H0.
+        * rewrite interp_state_vis in H0. apply vis_equ_bind in H0 as ?.
+          destruct H2 as [[] | (? & ? & ?)].
+          { rewrite H2 in H0. setoid_rewrite bind_ret_l in H0. step in H0. inv H0. }
+          pose proof (trans_vis e x x1). rewrite <- H2 in H4.
+          edestruct Hh. { destruct H5. rewrite H5 in H4. inv H4. }
+          destruct H5. rewrite H5 in H4.
+          specialize (H3 x). rewrite H5 in H2.
+          apply equ_vis_invT in H2 as ?. subst.
+          apply equ_vis_invE in H2 as ?. destruct H6 as [-> ?].
+          rewrite <- H6 in *. rewrite bind_ret_l in H3.
+          exists (k1 (snd x)), (fst x).
+          rewrite H in H3. split. { rewrite <- ctree_eta, H3. eright; eauto. eleft; auto. }
+          right.
+          exists x0. rewrite H1. split; etrans.
+          split; setoid_rewrite (ctree_eta (k0 x0)); setoid_rewrite Heqc.
+          { setoid_rewrite interp_state_vis. rewrite H5. setoid_rewrite bind_vis.
+            econstructor. rewrite bind_ret_l. rewrite <- H3, <- ctree_eta. reflexivity. }
+          eapply transis_obs; etrans. 2: { rewrite H5. etrans. } destruct x. now left.
+        * rewrite interp_state_br in H0. step in H0. inv H0.
+      + pose proof (trans_vis e x x0).
+        rewrite <- H1 in H3. edestruct Hpre.
+        { apply H4 in H3. inv H3. }
+        apply H4 in H3 as [].
+        specialize (H2 x).
+        exists (k0 x1), s. rewrite H in H2. split.
+        { rewrite <- ctree_eta, H2. eapply t0_det_bind_ret_l; eauto. now left. }
+        left. exists (obs e x), (x0 x), x1. split; auto. rewrite H1. etrans.
+    - exists stuckD, (fst r). split.
+      + left. unfold stuck. rewrite interp_state_br.
+        rewrite !br0_always_stuck.
+        rewrite bind_branch.
+        step.
+        constructor; intros [].
+      + right. symmetry in H0. apply ret_equ_bind in H0 as (? & ? & ?).
+        exists x. rewrite H. split; etrans. split.
+        rewrite H0. rewrite br0_always_stuck. etrans.
+        apply interp_state_ret_inv in H0 as []. subst. rewrite H0. destruct r. cbn. apply transis_val. econstructor; etrans.
+  Qed.
 
-Lemma trans_fold_state_inv {E F X} (h : E ~> stateT S (ctree F)) (Hh : forall X e s, vsimple (h X e s)) :
-  forall l (t : ctree E X) t' s,
-  trans l (fold_state h t s) t' ->
-  exists l t0 s', t0_det t' (fold_state h t0 s') /\ transi_state h l s s' t t0.
-Proof.
-  intros.
-   assert (trans l (Guard (Ret tt);; fold_state h t s) t').
-   { cbn. etrans. }
-  eapply trans_fold_state_inv_gen in H0; eauto. destruct H0 as (? & ? & ? & ?).
-  destruct H1 as [(? & ? & ? & ? & ? & ?) | (? & ? & ? & ?)].
-  - inv_trans. subst. inv H2. step in H1. inv H1. step in H3. inv H3.
-  - inv_trans. subst. eauto.
-  - left. intros. inv_trans. subst. constructor.
-Qed.
+  Lemma trans_interp_state_inv (Hh : forall X (e : _ X) s, vsimple (h e s)) :
+    forall l (t : ctree E C X) t' s,
+      trans l (interp_state h t s) t' ->
+      exists l t0 s', t0_det t' (interp_state h t0 s') /\ transi_state l s s' t t0.
+  Proof.
+    intros.
+    assert (trans l (Guard (Ret tt);; interp_state h t s) t').
+    { cbn. etrans. }
+    eapply trans_interp_state_inv_gen in H0; eauto. destruct H0 as (? & ? & ? & ?).
+    destruct H1 as [(? & ? & ? & ? & ? & ?) | (? & ? & ? & ?)].
+    - inv_trans. subst. inv H2. step in H1. inv H1. step in H3. inv H3.
+      exfalso; now apply void_unit_elim.
+    - inv_trans. subst. eauto.
+    - left. intros. inv_trans. subst. constructor.
+  Qed.
 
 (** The main theorem stating that fold_state preserves sbisim. *)
 
-Theorem fold_state_sbisim_gen {E F X Y} (h : E ~> stateT S (ctree F)) (Hh : forall X e s, vsimple (h X e s)) :
-  forall s (k k' : X -> ctree E Y) (pre pre' : ctree F X),
-  (forall x, sbisim (k x) (k' x)) ->
-  pre ≅ pre' ->
-  vsimple pre ->
-  sbisim (a <- pre;; Guard (fold_state h (k a) s)) (a <- pre';; Guard (fold_state h (k' a) s)).
-Proof.
-  revert X. coinduction R CH.
-  symmetric using idtac.
-  { intros. apply H; eauto.  intros. rewrite H0. reflexivity. now rewrite H1. red; now setoid_rewrite <- H1. }
-  assert (CH' : forall (t t' : ctree E Y) s, t ~ t' -> st R (fold_state h t s) (fold_state h t' s)).
-  {
-    intros.
-    assert (st R (a <- Ret tt;; Guard (fold_state h ((fun _ => t) a) s))
-      (a <- Ret tt;; Guard (fold_state h ((fun _ => t') a) s))).
-    { apply CH; eauto. left; eauto. }
-    setoid_rewrite bind_ret_l in H0.
-    rewrite !sb_guard in H0.
-    apply H0.
-  }
-  intros. setoid_rewrite <- H0. clear pre' H0. cbn. intros.
-  copy H0. rewrite bind_tau_r in H0.
-  eapply trans_fold_state_inv_gen in H0 as (? & ? & ? & ?); auto.
-  2: { destruct H1 as [[] | []]; rewrite H1.
-    rewrite bind_ret_l. apply is_simple_guard_ret.
-    rewrite bind_trigger. right. intros. inv_trans. subst.
-    exists x0. rewrite EQ. eright. left. reflexivity. reflexivity.
-  }
-  destruct H2.
-  - destruct H2 as (? & ? & ? & ? & ? & ?). rewrite H4 in H0. clear x H4.
-    destruct H1 as [[] | []].
-    + rewrite H1, bind_ret_l in H2. rewrite H1, bind_ret_l in cpy. inv_trans. subst.
-      inv H3. step in H2. inv H2. step in H4. inv H4.
-    + rewrite H1 in *. rewrite bind_trigger in H2. apply trans_vis_inv in H2 as (? & ? & ?). subst.
-      rewrite H2 in H3. inv H3. step in H4. inv H4.
-      apply equ_br_invE in H5. 2: apply Fin.F1.
-      rewrite <- H5 in H4. inv H4. 2: { step in H6. inv H6. }
-      step in H3. inv H3. clear x2 H2 t H5.
-      rewrite bind_trigger in cpy. apply trans_vis_inv in cpy. destruct cpy as (? & ? & ?). subst.
-      exists (Guard (fold_state h (k' x1) s)). rewrite H1. rewrite bind_trigger. now constructor.
-      rewrite H2, !sb_guard. apply CH'. apply H.
-  - destruct H2 as (? & ? & ? & ?).
-    destruct H1 as [[] | []]. 2: { rewrite H1 in H2. setoid_rewrite bind_trigger in H2. inv_trans. }
-    rewrite H1 in *. rewrite bind_ret_l in H2. inv_trans. subst. clear EQ.
-    eapply transis_sbisim in H4; eauto. destruct H4 as (? & ? & ?).
-    apply transis_trans in H2 as (? & ? & ?); auto.
-    exists x3. rewrite H1, bind_ret_l. etrans.
-    assert (st R (fold_state h x x0) (fold_state h x1 x0)).
-    { apply CH'. apply H4. }
-    rewrite sbisim_t0_det. 2: apply H0.
-    setoid_rewrite sbisim_t0_det at 3. 2: apply H5.
-    apply H6.
-Qed.
+  Theorem interp_state_sbisim_gen {Y} (Hh : forall X (e : _ X) s, vsimple (h e s)) :
+    forall s (k k' : Y -> ctree E C X) (pre pre' : ctree F D Y),
+      (forall x, sbisim eq (k x) (k' x)) ->
+      pre ≅ pre' ->
+      vsimple pre ->
+      sbisim eq (a <- pre;; Guard (interp_state h (k a) s)) (a <- pre';; Guard (interp_state h (k' a) s)).
+  Proof.
+    revert Y. coinduction R CH.
+    (* We would like to use a symmetry argument here, as is done in the 0.1 branch *)
+    assert (CH' : forall (t t' : ctree E C X) s, t ~ t' -> st eq R (interp_state h t s) (interp_state h t' s)).
+    {
+      intros.
+      assert (st eq R (a <- Ret tt;; Guard (interp_state h ((fun _ => t) a) s))
+                (a <- Ret tt;; Guard (interp_state h ((fun _ => t') a) s))).
+      { apply CH; eauto. left; eauto. }
+      setoid_rewrite bind_ret_l in H0.
+      rewrite !sb_guard in H0.
+      apply H0.
+    }
+    intros. setoid_rewrite <- H0. clear pre' H0. cbn.
+    split; cbn; intros.
+    - copy H0. rewrite bind_tau_r in H0.
+      eapply trans_interp_state_inv_gen in H0 as (? & ? & ? & ?); auto.
+      2: { destruct H1 as [[] | []]; rewrite H1.
+           rewrite bind_ret_l. apply is_simple_guard_ret.
+           rewrite bind_trigger. right. intros. inv_trans. subst.
+           exists x0. rewrite EQ. eright. left. reflexivity. reflexivity.
+      }
+      destruct H2.
+      + destruct H2 as (? & ? & ? & ? & ? & ?). rewrite H4 in H0. clear x H4.
+        destruct H1 as [[] | []].
+        * rewrite H1, bind_ret_l in H2. rewrite H1, bind_ret_l in cpy. inv_trans. subst.
+          inv H3. step in H2. inv H2. step in H4. inv H4.
+          exfalso; now apply void_unit_elim.
+        * rewrite H1 in *. rewrite bind_trigger in H2. apply trans_vis_inv in H2 as (? & ? & ?). subst.
+          rewrite H2 in H3. inv H3. step in H4. inv H4.
+          apply equ_br_invE in H5 as [_ ?].
+          rewrite <- H3 in H4; auto. inv H4.
+          2: { step in H6. inv H6. }
+          step in H5. inv H5.
+          rewrite bind_trigger in cpy. apply trans_vis_inv in cpy. destruct cpy as (? & ? & ?). subst.
+          eexists. exists (Guard (interp_state h (k' x1) s)). rewrite H1. rewrite bind_trigger. split.
+          now constructor.
+          split; auto.
+          rewrite H4, !sb_guard. apply CH'. apply H.
+      + destruct H2 as (? & ? & ? & ?).
+        destruct H1 as [[] | []].
+        2: { rewrite H1 in H2. setoid_rewrite bind_trigger in H2. inv_trans. }
+        rewrite H1 in *. rewrite bind_ret_l in H2. inv_trans. subst. clear EQ.
+        eapply transis_sbisim in H4; eauto. destruct H4 as (? & ? & ?).
+        apply transis_trans in H2 as (? & ? & ?); auto.
+        eexists; exists x3. rewrite H1, bind_ret_l. split.
+        etrans.
+        assert (st eq R (interp_state h x x0) (interp_state h x1 x0)).
+        { apply CH'. apply H4. }
+        split; auto.
+        rewrite sbisim_t0_det. 2: apply H0.
+        apply sbisim_t0_det in H5; rewrite H5.
+        apply H6.
+    - copy H0. rewrite bind_tau_r in H0.
+      eapply trans_interp_state_inv_gen in H0 as (? & ? & ? & ?); auto.
+      2: { destruct H1 as [[] | []]; rewrite H1.
+           rewrite bind_ret_l. apply is_simple_guard_ret.
+           rewrite bind_trigger. right. intros. inv_trans. subst.
+           exists x0. rewrite EQ. eright. left. reflexivity. reflexivity.
+      }
+      destruct H2.
+      + destruct H2 as (? & ? & ? & ? & ? & ?). rewrite H4 in H0. clear x H4.
+        destruct H1 as [[] | []].
+        * rewrite H1, bind_ret_l in H2. rewrite H1, bind_ret_l in cpy. inv_trans. subst.
+          inv H3. step in H2. inv H2. step in H4. inv H4.
+          exfalso; now apply void_unit_elim.
+        * rewrite H1 in *. rewrite bind_trigger in H2. apply trans_vis_inv in H2 as (? & ? & ?). subst.
+          rewrite H2 in H3. inv H3. step in H4. inv H4.
+          apply equ_br_invE in H5 as [_ ?].
+          rewrite <- H3 in H4; auto. inv H4.
+          2: { step in H6. inv H6. }
+          step in H5. inv H5.
+          rewrite bind_trigger in cpy. apply trans_vis_inv in cpy. destruct cpy as (? & ? & ?). subst.
+          eexists. exists (Guard (interp_state h (k x1) s)). rewrite H1. rewrite bind_trigger. split.
+          now constructor.
+          split; auto.
+          rewrite H4, !sb_guard. apply CH'. apply H.
+      + destruct H2 as (? & ? & ? & ?).
+        destruct H1 as [[] | []].
+        2: { rewrite H1 in H2. setoid_rewrite bind_trigger in H2. inv_trans. }
+        rewrite H1 in *. rewrite bind_ret_l in H2. inv_trans. subst. clear EQ.
+        eapply transis_sbisim in H4; [| symmetry; apply H]. destruct H4 as (? & ? & ?).
+        apply transis_trans in H2 as (? & ? & ?); auto.
+        exists l. exists x3. rewrite H1, bind_ret_l. split.
+        etrans.
+        assert (st eq R (interp_state h x x0) (interp_state h x1 x0)).
+        { apply CH'. apply H4. }
+        split; auto.
+        rewrite sbisim_t0_det. 2: apply H5.
+        apply sbisim_t0_det in H0; rewrite H0.
+        symmetry; apply H6.
+  Qed.
 
-#[global] Instance fold_state_sbisim {E F R} (h : E ~> stateT S (ctree F)) (Hh : forall X e s, vsimple (h X e s)) :
-  Proper (sbisim ==> eq ==> sbisim) (fold_state h (T := R)).
-Proof.
-  cbn. intros. subst.
-  assert (a <- Ret tt;; Guard (fold_state h ((fun _ => x) a) y0) ~
-    a <- Ret tt;; Guard (fold_state h ((fun _ => y) a) y0)).
-  apply fold_state_sbisim_gen; auto.
-  red; eauto.
-  setoid_rewrite bind_ret_l in H0. rewrite !sb_guard in H0. apply H0.
-Qed.
-   *)
+  #[global] Instance interp_state_sbisim (Hh : forall X (e : _ X) s, vsimple (h e s)) :
+    Proper (sbisim eq ==> eq ==> sbisim eq) (interp_state h (C := C) (T := X)).
+  Proof.
+    cbn. intros. subst.
+    assert (a <- Ret tt;; Guard (interp_state h ((fun _ => x) a) y0) ~
+                           a <- Ret tt;; Guard (interp_state h ((fun _ => y) a) y0)).
+    apply interp_state_sbisim_gen; auto.
+    red; eauto.
+    setoid_rewrite bind_ret_l in H0. rewrite !sb_guard in H0. apply H0.
+  Qed.
 
-(* End State. *)
+End transi_state.
 
 Arguments get {S E _}.
 Arguments put {S E _}.
 Arguments run_state {S E} [_] _ _.
 Arguments fold_state {E C M S FM MM IM} h g [T].
+Arguments interp_state {E C M S FM MM IM BM} h [T].
+Arguments refine_state {E C M S FM MM IM TM} g [T].
